experiment/Experiment.Steel.CondSolver.Test.fst
@@ -16,15 +16,15 @@ open Experiment.Steel.CondSolver
 
 
 let _ : elem_index #int 4 [1;3;4;2;7]
-  = _ by (build_elem_index ())
+  = _ by (build_elem_index dummy_ctx)
 
 [@@ expect_failure [228]]
 let _ : elem_index #int 5 [1;3;4;2;7]
-  = _ by (build_elem_index ())
+  = _ by (build_elem_index dummy_ctx)
 
 [@@ expect_failure [228]]
 let _ : elem_index #int 4 L.(0 :: ([1;3] @ [4;2;7]))
-  = _ by (build_elem_index ())
+  = _ by (build_elem_index dummy_ctx)
 
 unfold
 let specT (a : Type) (pre : M.pre_t) (post : M.post_t a) : M.prog_tree a
