experiment/Experiment.Steel.Interface.fst
@@ -1,0 +1,87 @@
+module Experiment.Steel.Interface
+
+module L = FStar.List.Pure
+
+open FStar.Tactics
+
+
+type stage =
+  | Stage_M
+  | Stage_ST
+  | Stage_SF
+  | Stage_Fun
+  | Stage_WP
+
+type flag =
+  | Timer
+  | Dump of stage
+
+noeq
+type flags_record = {
+  f_timer : bool;
+  f_dump  : stage -> bool;
+}
+
+let default_flags : flags_record = {
+  f_timer = false;
+  f_dump  = (fun _ -> false);
+}
+
+let record_flag (r : flags_record) (f : flag) : flags_record =
+  match f with
+  | Timer  -> {r with f_timer = true}
+  | Dump s -> {r with f_dump  = (fun s' -> s' = s || r.f_dump s')}
+
+let make_flags_record : list flag -> flags_record =
+  L.fold_left record_flag default_flags
+
+
+type failure_goal_shape =
+  | GShape_truth_refl_list
+  | GShape_vprop
+  | GShape_tree_cond
+
+noeq
+type failure_enum =
+  | Fail_goal_shape : (expected : failure_goal_shape) -> failure_enum
+  | Fail_post_unification
+  | Fail_cond_sol
+  | Fail_elem_index
+  | Fail_shape_unification : nat -> nat -> failure_enum
+
+noeq
+type info =
+  | Info_goal : typ -> info
+  | Info_original_exn : exn -> info
+  | Info_location : string -> info
+
+noeq
+type failure_t = {
+  fail_enum : failure_enum;
+  fail_info : list info
+}
+
+exception Failure of failure_t
+
+let info_to_string (i : info) : Tac string =
+  match i with
+  | Info_goal g -> "on goal: "^term_to_string g
+  | Info_original_exn exn ->
+      begin match exn with
+      | TacticFailure msg -> "original failure: "^msg
+      | exn -> "original exception: "^term_to_string (quote exn)
+      end
+  | Info_location s -> s
+
+private
+let rec concat_sep (sep : string) (l : list string)
+  : Tot string (decreases l)
+  = match l with
+  | []  -> ""
+  | [x] -> x
+  | x :: y :: tl -> x^sep^concat_sep sep (y :: tl)
+
+let failure_to_string (f : failure_t) : Tac string =
+  let enum = f.fail_enum in
+  let msg = term_to_string (quote enum) in
+  concat_sep "\n" (msg :: map info_to_string f.fail_info)
