experiment/Experiment.Steel.Notations.fst
@@ -1,0 +1,51 @@
+module Experiment.Steel.Notations
+
+include Experiment.Steel.Interface
+
+module M  = Experiment.Steel.Repr.M
+module SE = Steel.Effect
+
+open FStar.Tactics
+open Experiment.Steel
+
+
+unfold
+let steel
+  : (a : Type) -> (pre : SE.pre_t) -> (post : SE.post_t a) ->
+    (req : SE.req_t pre) -> (ens : SE.ens_t pre a post) -> Type
+  = M.unit_steel
+
+unfold
+let to_steel
+      (#a : Type) (#pre : SE.pre_t) (#post : SE.post_t a) (#req : SE.req_t pre) (#ens : SE.ens_t pre a post)
+      (t : M.repr a)
+      (g : __to_steel_goal a pre post req ens t)
+  : M.unit_steel a pre post req ens
+  = to_steel #a #pre #post #req #ens t g
+
+let mk_steel (fs : list flag) : Tac unit
+  = build_to_steel (make_flags_record fs)
+
+
+unfold
+let return_hint (#a : Type) (x : a) (sl_hint : M.post_t a)
+  : M.repr a
+  = M.return_hint #a x sl_hint
+
+unfold
+let return (#a : Type) (x : a)
+  : M.repr a
+  = M.return #a x
+
+unfold
+let bind (#a #b : Type) (f : M.repr a) (g : a -> M.repr b)
+  : M.repr b
+  = M.bind #a #b f g
+
+unfold
+let call (#b : Type)
+      (#a : b -> Type) (#pre : b -> SE.pre_t) (#post : (x : b) -> SE.post_t (a x))
+      (#req : (x : b) -> SE.req_t (pre x)) (#ens : (x : b) -> SE.ens_t (pre x) (a x) (post x))
+      ($f : (x : b) -> SE.Steel (a x) (pre x) (post x) (req x) (ens x)) (x : b)
+  : M.repr (a x)
+  = M.repr_of_steel (pre x) (post x) (req x) (ens x) (fun () -> f x)
